abs1_comb_thm/comb_abs1_hold_ref_rel_WR_UPScript.sml
@@ -1,5 +1,5 @@
 open HolKernel bossLib boolLib Parse wordsLib pred_setLib;
-open SPI_stateTheory SPI_relationTheory SPI_update_regsTheory driver_stateTheory driver_relationTheory driver_writeTheory ds_abs1_stateTheory ds_abs1_relTheory ds_abs1_initTheory ds_abs1_txTheory ds_abs1_rxTheory ds_abs1_xferTheory ref_relTheory board_memTheory;
+open SPI_stateTheory SPI_relationTheory SPI_update_regsTheory SPI_return_regsTheory driver_stateTheory driver_relationTheory driver_writeTheory ds_abs1_stateTheory ds_abs1_relTheory ds_abs1_initTheory ds_abs1_txTheory ds_abs1_rxTheory ds_abs1_xferTheory ref_relTheory board_memTheory;
 
 val _ = new_theory "comb_abs1_hold_ref_rel_WR_UP";
 
@@ -19,7 +19,8 @@ Cases_on `dr.state` >> rw [] >>
 Cases_on `ds_abs1.state` >> rw [] >>
 Cases_on `spi.state` >> rw [] >>
 rw [write_SYSCONFIG_comb_def, write_SOFTRESET_def] >>
-fs [ref_rel_def, IS_STATE_REL_def]);
+fs [ref_rel_def, IS_STATE_REL_def] >>
+METIS_TAC []);
 
 
 (* relation holds for ds_abs1 or ds_abs1' when driver state is dr_init_setting *)
@@ -31,20 +32,9 @@ val ref_rel_hold_dr_init_setting_WR = store_thm("ref_rel_hold_dr_init_setting_WR
 (?ds_abs1'. (ds_abs1_tr ds_abs1 tau ds_abs1') /\ 
 (ref_rel ds_abs1' ((dr_write_state dr), spi')))``,
 rw [spi_tr_cases] >>
-rw [dr_write_state_def, dr_write_address_def, dr_write_value_def,dr_write_def] >|
-[ (* update SYSCONFIG *)
-rw [dr_write_sysconfig_def, write_SPI_regs_def, SPI0_SYSCONFIG_def, SPI0_PA_RANGE_def,SPI0_START_def, SPI0_END_def] >|
-[DISJ2_TAC >>
-`IS_STATE_REL ds_abs1 dr spi` by fs [ref_rel_def] >>
-fs [IS_STATE_REL_def] >>
-Cases_on `dr.state` >> rw [] >>
-Cases_on `ds_abs1.state` >> rw [] >>
-Cases_on `spi.state` >> rw [] >>
-rw [ds_abs1_tr_cases, ds_abs1_comb_tr_cases] >>
-EXISTS_TAC ``comb_abs1_init_operations ds_abs1`` >>
-rw [COMB_ABS1_INIT_ENABLE_def, write_SYSCONFIG_comb_def, write_SYSCONFIG_def, 
-comb_abs1_init_operations_def, comb_abs1_init_start_op_def] >>
-fs [ref_rel_def, IS_STATE_REL_def],
+rw [dr_write_state_def, dr_write_address_def, dr_write_value_def,dr_write_def] >| [
+(* update SYSCONFIG *)
+rw [dr_write_sysconfig_def, write_SPI_regs_def, SPI0_SYSCONFIG_def, SPI0_PA_RANGE_def,SPI0_START_def, SPI0_END_def] >>
 DISJ1_TAC >>
 rw [write_SYSCONFIG_comb_def, write_SYSCONFIG_def] >|
 [METIS_TAC [ref_rel_def],
@@ -54,104 +44,46 @@ METIS_TAC [],
 fs [IS_STATE_REL_def] >>
 Cases_on `dr.state` >> rw [] >>
 Cases_on `ds_abs1.state` >> rw [] >>
-Cases_on `spi.state` >> rw []]],
+Cases_on `spi.state` >> rw []],
 (* update MODULCTRL *)
 rw [dr_write_modulctrl_def, write_SPI_regs_def, SPI0_MODULCTRL_def, SPI0_SYSCONFIG_def, 
-SPI0_PA_RANGE_def, SPI0_START_def, SPI0_END_def] >|
-[DISJ2_TAC >>
+SPI0_PA_RANGE_def, SPI0_START_def, SPI0_END_def] >>
+DISJ1_TAC >>
 `IS_STATE_REL ds_abs1 dr spi` by fs [ref_rel_def] >>
 fs [IS_STATE_REL_def] >>
 Cases_on `dr.state` >> rw [] >>
 Cases_on `ds_abs1.state` >> rw [] >>
-Cases_on `spi.state` >> rw [] >>
-rw [ds_abs1_tr_cases, ds_abs1_comb_tr_cases] >>
-EXISTS_TAC ``comb_abs1_init_operations ds_abs1`` >>
-rw [COMB_ABS1_INIT_ENABLE_def, write_MODULCTRL_def, comb_abs1_init_operations_def, 
-comb_abs1_init_start_op_def] >>
-fs [ref_rel_def, IS_STATE_REL_def],
-DISJ1_TAC >>
-rw [write_MODULCTRL_def] >|
-[METIS_TAC [ref_rel_def],
+Cases_on `spi.state` >> rw [write_MODULCTRL_def] >-
+(`spi.regs.CH0CONF.WL = 0w` by fs [ref_rel_def] >>
+`~(0w:word5 >+ 2w:word5)` by EVAL_TAC >>
+fs []) >>
 fs [ref_rel_def, IS_STATE_REL_def] >>
 METIS_TAC [],
-`IS_STATE_REL ds_abs1 dr spi` by fs [ref_rel_def] >>
-fs [IS_STATE_REL_def] >>
-Cases_on `dr.state` >> rw [] >>
-Cases_on `ds_abs1.state` >> rw [] >>
-Cases_on `spi.state` >> rw []]],
-(* update CH0CONF.WL *)
-rw [dr_write_ch0conf_wl_def, write_SPI_regs_def, SPI0_CH0CONF_def, SPI0_MODULCTRL_def, 
-SPI0_SYSCONFIG_def, SPI0_PA_RANGE_def, SPI0_START_def, SPI0_END_def] >|
-[DISJ2_TAC >>
-`IS_STATE_REL ds_abs1 dr spi` by fs [ref_rel_def] >>
-fs [IS_STATE_REL_def] >> rw [] >>
-Cases_on `dr.state` >> rw [] >>
-Cases_on `ds_abs1.state` >> rw [] >>
-Cases_on `spi.state` >> rw [] >>
-rw [ds_abs1_tr_cases, ds_abs1_comb_tr_cases] >>
-EXISTS_TAC ``comb_abs1_init_operations ds_abs1`` >>
-rw [COMB_ABS1_INIT_ENABLE_def, write_CH0CONF_comb_def, write_CH0CONF_WL_def,
-comb_abs1_init_operations_def, comb_abs1_init_start_op_def] >> 
-fs [ref_rel_def, IS_STATE_REL_def] >>
-UNDISCH_TAC ``~(7w:word5 >+ 2w:word5)`` >>
-EVAL_TAC,
-DISJ1_TAC >>
-rw [write_CH0CONF_comb_def, write_CH0CONF_WL_def] >|
-[METIS_TAC [ref_rel_def],
-fs [ref_rel_def, IS_STATE_REL_def] >>
-METIS_TAC [],
-`IS_STATE_REL ds_abs1 dr spi` by fs [ref_rel_def] >>
-fs [IS_STATE_REL_def] >>
-Cases_on `dr.state` >> rw [] >>
-Cases_on `ds_abs1.state` >> rw [] >>
-Cases_on `spi.state` >> rw [] >>
-UNDISCH_TAC ``~(7w:word5 >+ 2w:word5)`` >>
-EVAL_TAC]],
-(* update CH0CONF.IS,DPE,TRM etc bits *)
-rw [dr_write_ch0conf_mode_def, write_SPI_regs_def, SPI0_CH0CONF_def, SPI0_MODULCTRL_def, 
-SPI0_SYSCONFIG_def, SPI0_PA_RANGE_def, SPI0_START_def, SPI0_END_def] >|
-[DISJ2_TAC >>
-`IS_STATE_REL ds_abs1 dr spi` by fs [ref_rel_def] >>
-fs [IS_STATE_REL_def] >>
-Cases_on `dr.state` >> rw [] >>
-Cases_on `ds_abs1.state` >> rw [] >>
-Cases_on `spi.state` >> rw [] >>
-rw [ds_abs1_tr_cases, ds_abs1_comb_tr_cases] >>
-EXISTS_TAC ``comb_abs1_init_operations ds_abs1`` >>
-rw [COMB_ABS1_INIT_ENABLE_def, write_CH0CONF_comb_def, write_CH0CONF_def,
-comb_abs1_init_operations_def, comb_abs1_init_start_op_def] >>
-fs [ref_rel_def, IS_STATE_REL_def],
-DISJ1_TAC >>
-rw [write_CH0CONF_comb_def, write_CH0CONF_def] >|
-[METIS_TAC [ref_rel_def],
-fs [ref_rel_def, IS_STATE_REL_def] >>
-METIS_TAC [],
-`IS_STATE_REL ds_abs1 dr spi` by fs [ref_rel_def] >>
-fs [IS_STATE_REL_def] >>
-Cases_on `dr.state` >> rw [] >>
-Cases_on `ds_abs1.state` >> rw [] >>
-Cases_on `spi.state` >> rw []]],
-(* update CH0CONF.CLKD *)
-rw [dr_write_ch0conf_speed_def, write_SPI_regs_def, SPI0_CH0CONF_def, SPI0_MODULCTRL_def, 
+(* update CH0CONF *)
+rw [dr_write_ch0conf_init_def, write_SPI_regs_def, SPI0_CH0CONF_def, SPI0_MODULCTRL_def, 
 SPI0_SYSCONFIG_def, SPI0_PA_RANGE_def, SPI0_START_def, SPI0_END_def] >>
-DISJ2_TAC >>
 `IS_STATE_REL ds_abs1 dr spi` by fs [ref_rel_def] >>
 fs [IS_STATE_REL_def] >>
 Cases_on `dr.state` >> rw [] >>
 Cases_on `ds_abs1.state` >> rw [] >>
 Cases_on `spi.state` >> rw [] >>
+`spi.regs.CH0CONF.IS = 1w /\ spi.regs.CH0CONF.FORCE = 0w` by fs [ref_rel_def] >>
+`(19 >< 19) (66523w:word32):word1 <> spi.regs.CH0CONF.IS` 
+by FULL_SIMP_TAC (std_ss++WORD_ss) [] >>
+`ch0conf_changed (66523w:word32) spi` by fs [ch0conf_changed_def] >>
+rw [write_CH0CONF_comb_def, write_CH0CONF_init_def] >-
+(DISJ2_TAC >>
 rw [ds_abs1_tr_cases, ds_abs1_comb_tr_cases] >>
 EXISTS_TAC ``comb_abs1_init_operations ds_abs1`` >>
-rw [COMB_ABS1_INIT_ENABLE_def, write_CH0CONF_comb_def, write_CH0CONF_speed_def,
-comb_abs1_init_operations_def, comb_abs1_init_start_op_def] >>
-fs [ref_rel_def, IS_STATE_REL_def] >>
+rw [COMB_ABS1_INIT_ENABLE_def,comb_abs1_init_operations_def, comb_abs1_init_start_op_def] >>
+fs [ref_rel_def, IS_STATE_REL_def]) >>
+`7w:word5 >+ 2w:word5` by EVAL_TAC >>
 METIS_TAC [ref_rel_def]]);
 
-
-(* relation holds when driver state is dr_tx_idle *)
-val ref_rel_hold_dr_tx_idle_WR = store_thm("ref_rel_hold_dr_tx_idle_WR",
+(* relation holds when driver state is dr_tx_fetch_conf *)
+val ref_rel_hold_dr_tx_fetch_conf_WR = store_thm("ref_rel_hold_dr_tx_fetch_conf_WR",
 ``!(spi:spi_state) (dr:driver_state) (ds_abs1:ds_abs1_state) (spi':spi_state).
-(ref_rel ds_abs1 (dr, spi)) /\ (dr.state = dr_tx_idle) /\
+(ref_rel ds_abs1 (dr, spi)) /\ (dr.state = dr_tx_fetch_conf) /\
 (spi_tr spi (Update (THE (dr_write_address dr)) (THE (dr_write_value dr))) spi') ==>
 ref_rel ds_abs1 ((dr_write_state dr), spi')``,
 rw [spi_tr_cases] >>
@@ -163,7 +95,17 @@ fs [IS_STATE_REL_def] >>
 Cases_on `dr.state` >> rw [] >>
 Cases_on `ds_abs1.state` >> rw [] >>
 Cases_on `spi.state` >> rw [] >>
+`dr.dr_last_read_v = SOME (build_CH0CONF spi.regs.CH0CONF)` by fs [ref_rel_def] >>
+`~ (ch0conf_changed ((4293906431w:word32) && (build_CH0CONF spi.regs.CH0CONF) || 
+(1056768w:word32)) spi)` by (fs [build_CH0CONF_def,ch0conf_changed_def] >>
+FULL_SIMP_TAC (std_ss++WORD_ss++WORD_BIT_EQ_ss) []) >>
+`spi.regs.CH0CONF.FORCE = 0w` by fs [ref_rel_def] >>
+`(20 >< 20) ((4293906431w:word32) && (build_CH0CONF spi.regs.CH0CONF) || 
+(1056768w:word32)) : word1 <> spi.regs.CH0CONF.FORCE` by FULL_SIMP_TAC (std_ss++WORD_ss++WORD_BIT_EQ_ss) [] >>
+`(13 >< 12) ((4293906431w:word32) && (build_CH0CONF spi.regs.CH0CONF) || 
+(1056768w:word32)) : word2 = 2w` by FULL_SIMP_TAC (std_ss++WORD_ss++WORD_BIT_EQ_ss) [] >>
 rw [write_CH0CONF_comb_def, write_CH0CONF_tx_def] >>
+FULL_SIMP_TAC (std_ss++WORD_ss++WORD_BIT_EQ_ss) [] >>
 fs [ref_rel_def, IS_STATE_REL_def]);
 
 (* relation holds when driver state is dr_tx_conf_issued *)
@@ -274,14 +216,21 @@ rw [COMB_ABS1_TX_ENABLE_def] >>
 rw [comb_abs1_tx_operations_def, comb_abs1_tx_reset_op_def, dr_write_state_def, 
 dr_write_value_def,dr_write_address_def, dr_write_def, dr_write_ch0conf_tx_def, 
 write_SPI_regs_def, SPI0_SYSCONFIG_def, SPI0_PA_RANGE_def, SPI0_START_def, 
-SPI0_END_def, SPI0_CH0CONF_def, SPI0_MODULCTRL_def, write_CH0CONF_comb_def, 
-write_CH0CONF_tx_def] >>
+SPI0_END_def, SPI0_CH0CONF_def, SPI0_MODULCTRL_def] >> 
+`dr.dr_last_read_v = SOME (build_CH0CONF spi.regs.CH0CONF)` by fs [ref_rel_def] >>
+`~ (ch0conf_changed ((4293918719w:word32) && (build_CH0CONF spi.regs.CH0CONF)) spi)` by (fs [build_CH0CONF_def,ch0conf_changed_def] >>
+FULL_SIMP_TAC (std_ss++WORD_ss++WORD_BIT_EQ_ss) []) >>
+`spi.regs.CH0CONF.FORCE = 1w` by fs [ref_rel_def] >>
+`(20 >< 20) ((4293918719w:word32) && (build_CH0CONF spi.regs.CH0CONF)) :word1 <> spi.regs.CH0CONF.FORCE` by FULL_SIMP_TAC (std_ss++WORD_ss++WORD_BIT_EQ_ss) [] >>
+`(13 >< 12) ((4293918719w:word32) && (build_CH0CONF spi.regs.CH0CONF)): word2 = spi.regs.CH0CONF.TRM` by (fs [build_CH0CONF_def] >> FULL_SIMP_TAC (std_ss++WORD_ss++WORD_BIT_EQ_ss) []) >>
+rw [write_CH0CONF_comb_def,write_CH0CONF_tx_def] >>
+FULL_SIMP_TAC (std_ss++WORD_ss++WORD_BIT_EQ_ss) [] >>
 fs [ref_rel_def, IS_STATE_REL_def]);
 
-(* relation holds when driver state is dr_rx_idle *)
-val ref_rel_hold_dr_rx_idle_WR = store_thm("ref_rel_hold_dr_rx_idle_WR",
+(* relation holds when driver state is dr_rx_fetch_conf *)
+val ref_rel_hold_dr_rx_fetch_conf_WR = store_thm("ref_rel_hold_dr_rx_fetch_conf_WR",
 ``!(spi:spi_state) (dr:driver_state) (ds_abs1:ds_abs1_state) (spi':spi_state).
-(ref_rel ds_abs1 (dr, spi)) /\ (dr.state = dr_rx_idle) /\
+(ref_rel ds_abs1 (dr, spi)) /\ (dr.state = dr_rx_fetch_conf) /\
 (spi_tr spi (Update (THE (dr_write_address dr)) (THE (dr_write_value dr))) spi') ==>
 ref_rel ds_abs1 ((dr_write_state dr), spi')``,
 rw [spi_tr_cases] >>
@@ -293,7 +242,17 @@ fs [IS_STATE_REL_def] >> rw [] >>
 Cases_on `dr.state` >> rw [] >>
 Cases_on `ds_abs1.state` >> rw [] >>
 Cases_on `spi.state` >> rw [] >>
+`dr.dr_last_read_v = SOME (build_CH0CONF spi.regs.CH0CONF)` by fs [ref_rel_def] >>
+`~ (ch0conf_changed ((4293906431w:word32) && (build_CH0CONF spi.regs.CH0CONF) || 
+(1052672w:word32)) spi)` by (fs [build_CH0CONF_def,ch0conf_changed_def] >>
+FULL_SIMP_TAC (std_ss++WORD_ss++WORD_BIT_EQ_ss) []) >>
+`spi.regs.CH0CONF.FORCE = 0w` by fs [ref_rel_def] >>
+`(20 >< 20) ((4293906431w:word32) && (build_CH0CONF spi.regs.CH0CONF) || 
+(1052672w:word32)) : word1 <> spi.regs.CH0CONF.FORCE` by FULL_SIMP_TAC (std_ss++WORD_ss++WORD_BIT_EQ_ss) [] >>
+`(13 >< 12) ((4293906431w:word32) && (build_CH0CONF spi.regs.CH0CONF) || 
+(1052672w:word32)) :word2 = 1w` by FULL_SIMP_TAC (std_ss++WORD_ss++WORD_BIT_EQ_ss) [] >>
 rw [write_CH0CONF_comb_def, write_CH0CONF_rx_def] >>
+FULL_SIMP_TAC (std_ss++WORD_ss++WORD_BIT_EQ_ss) [] >>
 fs [ref_rel_def, IS_STATE_REL_def]);
 
 (* relation holds when driver state is dr_rx_conf_issued *)
@@ -353,13 +312,20 @@ rw [comb_abs1_rx_operations_def, comb_abs1_rx_reset_op_def, dr_write_state_def,
 dr_write_value_def,dr_write_address_def, dr_write_def, dr_write_ch0conf_rx_def, 
 write_SPI_regs_def, SPI0_SYSCONFIG_def, SPI0_PA_RANGE_def, SPI0_START_def, 
 SPI0_END_def, SPI0_CH0CONF_def, SPI0_MODULCTRL_def] >>
+`dr.dr_last_read_v = SOME (build_CH0CONF spi.regs.CH0CONF)` by fs [ref_rel_def] >>
+`~ (ch0conf_changed ((4293918719w:word32) && (build_CH0CONF spi.regs.CH0CONF)) spi)` by (fs [build_CH0CONF_def,ch0conf_changed_def] >>
+FULL_SIMP_TAC (std_ss++WORD_ss++WORD_BIT_EQ_ss) []) >>
+`spi.regs.CH0CONF.FORCE = 1w` by fs [ref_rel_def] >>
+`(20 >< 20) ((4293918719w:word32) && (build_CH0CONF spi.regs.CH0CONF)) :word1 <> spi.regs.CH0CONF.FORCE` by FULL_SIMP_TAC (std_ss++WORD_ss++WORD_BIT_EQ_ss) [] >>
+`(13 >< 12) ((4293918719w:word32) && (build_CH0CONF spi.regs.CH0CONF)): word2 = spi.regs.CH0CONF.TRM` by (fs [build_CH0CONF_def] >> FULL_SIMP_TAC (std_ss++WORD_ss++WORD_BIT_EQ_ss) []) >>
 rw [write_CH0CONF_comb_def, write_CH0CONF_rx_def] >>
+FULL_SIMP_TAC (std_ss++WORD_ss++WORD_BIT_EQ_ss) [] >>
 fs [ref_rel_def, IS_STATE_REL_def]);
 
 (* relation holds when driver state is dr_xfer_idle *)
-val ref_rel_hold_dr_xfer_idle_WR = store_thm("ref_rel_hold_dr_xfer_idle_WR",
+val ref_rel_hold_dr_xfer_fetch_conf_WR = store_thm("ref_rel_hold_dr_xfer_fetch_conf_WR",
 ``!(spi:spi_state) (dr:driver_state) (ds_abs1:ds_abs1_state) (spi':spi_state).
-(ref_rel ds_abs1 (dr, spi)) /\ (dr.state = dr_xfer_idle) /\
+(ref_rel ds_abs1 (dr, spi)) /\ (dr.state = dr_xfer_fetch_conf) /\
 (spi_tr spi (Update (THE (dr_write_address dr)) (THE (dr_write_value dr))) spi') ==>
 ref_rel ds_abs1 ((dr_write_state dr), spi')``,
 rw [spi_tr_cases] >>
@@ -371,7 +337,17 @@ fs [IS_STATE_REL_def] >>
 Cases_on `dr.state` >> rw [] >>
 Cases_on `ds_abs1.state` >> rw [] >>
 Cases_on `spi.state` >> rw [] >>
+`dr.dr_last_read_v = SOME (build_CH0CONF spi.regs.CH0CONF)` by fs [ref_rel_def] >>
+`~ (ch0conf_changed ((4293906431w:word32) && (build_CH0CONF spi.regs.CH0CONF) || 
+(1048576w:word32)) spi)` by (fs [build_CH0CONF_def,ch0conf_changed_def] >>
+FULL_SIMP_TAC (std_ss++WORD_ss++WORD_BIT_EQ_ss) []) >>
+`spi.regs.CH0CONF.FORCE = 0w` by fs [ref_rel_def] >>
+`(20 >< 20) ((4293906431w:word32) && (build_CH0CONF spi.regs.CH0CONF) || 
+(1048576w:word32)) : word1 <> spi.regs.CH0CONF.FORCE` by FULL_SIMP_TAC (std_ss++WORD_ss++WORD_BIT_EQ_ss) [] >>
+`(13 >< 12) ((4293906431w:word32) && (build_CH0CONF spi.regs.CH0CONF) || 
+(1048576w:word32)) :word2 = 0w` by FULL_SIMP_TAC (std_ss++WORD_ss++WORD_BIT_EQ_ss) [] >>
 rw [write_CH0CONF_comb_def, write_CH0CONF_xfer_def] >>
+FULL_SIMP_TAC (std_ss++WORD_ss++WORD_BIT_EQ_ss) [] >>
 fs [ref_rel_def, IS_STATE_REL_def]);
 
 (* relation holds when driver state is dr_xfer_conf_issued *)
@@ -453,7 +429,16 @@ rw [COMB_ABS1_XFER_ENABLE_def] >>
 rw [comb_abs1_xfer_operations_def, comb_abs1_xfer_reset_op_def, dr_write_state_def, 
 dr_write_value_def,dr_write_address_def, dr_write_def, dr_write_ch0conf_xfer_def, 
 write_SPI_regs_def, SPI0_SYSCONFIG_def, SPI0_PA_RANGE_def, SPI0_START_def, 
-SPI0_END_def, SPI0_CH0CONF_def,SPI0_MODULCTRL_def, write_CH0CONF_comb_def, write_CH0CONF_xfer_def] >>
+SPI0_END_def, SPI0_CH0CONF_def,SPI0_MODULCTRL_def] >>
+`dr.dr_last_read_v = SOME (build_CH0CONF spi.regs.CH0CONF)` by fs [ref_rel_def] >>
+`~ (ch0conf_changed ((4293918719w:word32) && (build_CH0CONF spi.regs.CH0CONF)) spi)` 
+by (fs [build_CH0CONF_def,ch0conf_changed_def] >>
+FULL_SIMP_TAC (std_ss++WORD_ss++WORD_BIT_EQ_ss) []) >>
+`spi.regs.CH0CONF.FORCE = 1w` by fs [ref_rel_def] >>
+`(20 >< 20) ((4293918719w:word32) && (build_CH0CONF spi.regs.CH0CONF)) :word1 <> spi.regs.CH0CONF.FORCE` by FULL_SIMP_TAC (std_ss++WORD_ss++WORD_BIT_EQ_ss) [] >>
+`(13 >< 12) ((4293918719w:word32) && (build_CH0CONF spi.regs.CH0CONF)): word2 = spi.regs.CH0CONF.TRM` by (fs [build_CH0CONF_def] >> FULL_SIMP_TAC (std_ss++WORD_ss++WORD_BIT_EQ_ss) []) >>
+rw [write_CH0CONF_comb_def, write_CH0CONF_xfer_def] >>
+FULL_SIMP_TAC (std_ss++WORD_ss++WORD_BIT_EQ_ss) [] >>
 fs [ref_rel_def, IS_STATE_REL_def]);
 
 (* simulation: ref_rel holds for ds_abs1 or ds_abs1' when driver and controller perform WRITE and UPDATE operations *)
@@ -468,16 +453,16 @@ val comb_abs1_hold_ref_rel_WR_UP = store_thm("comb_abs1_hold_ref_rel_WR_UP",
 rw [driver_tr_cases, DR_WR_ENABLE_def] >|
 [METIS_TAC [ref_rel_hold_dr_init_idle_WR],
 METIS_TAC [ref_rel_hold_dr_init_setting_WR],
-METIS_TAC [ref_rel_hold_dr_tx_idle_WR],
+METIS_TAC [ref_rel_hold_dr_tx_fetch_conf_WR],
 METIS_TAC [ref_rel_hold_dr_tx_conf_issued_WR],
 METIS_TAC [ref_rel_hold_dr_tx_write_data_WR],
 METIS_TAC [ref_rel_hold_dr_tx_issue_disable_WR],
 METIS_TAC [ref_rel_hold_dr_tx_reset_conf_WR],
-METIS_TAC [ref_rel_hold_dr_rx_idle_WR],
+METIS_TAC [ref_rel_hold_dr_rx_fetch_conf_WR],
 METIS_TAC [ref_rel_hold_dr_rx_conf_issued_WR],
 METIS_TAC [ref_rel_hold_dr_rx_issue_disable_WR],
 METIS_TAC [ref_rel_hold_dr_rx_reset_conf_WR],
-METIS_TAC [ref_rel_hold_dr_xfer_idle_WR],
+METIS_TAC [ref_rel_hold_dr_xfer_fetch_conf_WR],
 METIS_TAC [ref_rel_hold_dr_xfer_conf_issued_WR],
 METIS_TAC [ref_rel_hold_dr_xfer_write_dataO_WR],
 METIS_TAC [ref_rel_hold_dr_xfer_issue_disable_WR],
