ds_abs1/ref_relScript.sml
@@ -1,6 +1,6 @@
 open HolKernel bossLib boolLib Parse;
 open wordsTheory listTheory;
-open SPI_stateTheory driver_stateTheory ds_abs1_stateTheory board_memTheory;
+open SPI_stateTheory SPI_return_regsTheory driver_stateTheory ds_abs1_stateTheory board_memTheory;
 
 val _ = new_theory "ref_rel";
 
@@ -21,6 +21,7 @@ IS_STATE_REL (ds_abs1:ds_abs1_state) (dr:driver_state) (spi:spi_state) =
 (dr.state = dr_ready /\ spi.state = spi_ready)) /\
 ((ds_abs1.state = abs1_tx_idle) =
 ((dr.state = dr_tx_idle /\ spi.state = spi_ready) \/
+(dr.state = dr_tx_fetch_conf /\ spi.state = spi_ready) \/
 (dr.state = dr_tx_conf_issued /\ spi.state = tx_conf_ready) \/
 (dr.state = dr_tx_read_txs /\ spi.state = tx_channel_enabled) \/
 (dr.state = dr_tx_check_txs /\ spi.state = tx_channel_enabled))) /\
@@ -57,9 +58,11 @@ IS_STATE_REL (ds_abs1:ds_abs1_state) (dr:driver_state) (spi:spi_state) =
 ((dr.state = dr_tx_read_eot /\ spi.state = tx_ready_for_trans) \/
 (dr.state = dr_tx_check_eot /\ spi.state = tx_ready_for_trans) \/
 (dr.state = dr_tx_issue_disable /\ spi.state = tx_ready_for_trans) \/
+(dr.state = dr_tx_read_conf /\ spi.state = tx_channel_disabled) \/
 (dr.state = dr_tx_reset_conf /\ spi.state = tx_channel_disabled))) /\
 ((ds_abs1.state = abs1_rx_idle) =
 ((dr.state = dr_rx_idle /\ spi.state = spi_ready) \/
+(dr.state = dr_rx_fetch_conf /\ spi.state = spi_ready) \/
 (dr.state = dr_rx_conf_issued /\ spi.state = rx_conf_ready) \/
 (dr.state = dr_rx_read_rxs /\ spi.state = rx_channel_enabled) \/
 (dr.state = dr_rx_check_rxs /\ spi.state = rx_channel_enabled))) /\
@@ -82,9 +85,11 @@ IS_STATE_REL (ds_abs1:ds_abs1_state) (dr:driver_state) (spi:spi_state) =
 (dr.state = dr_rx_fetch_data /\ spi.state = rx_data_ready)) /\
 ((ds_abs1.state = abs1_rx_reset) =
 ((dr.state = dr_rx_issue_disable /\ spi.state = rx_data_ready) \/
+(dr.state = dr_rx_read_conf /\ spi.state = rx_channel_disabled) \/
 (dr.state = dr_rx_reset_conf /\ spi.state = rx_channel_disabled))) /\
 ((ds_abs1.state = abs1_xfer_idle) =
 ((dr.state = dr_xfer_idle /\ spi.state = spi_ready) \/
+(dr.state = dr_xfer_fetch_conf /\ spi.state = spi_ready) \/
 (dr.state = dr_xfer_conf_issued /\ spi.state = xfer_conf_ready) \/
 (dr.state = dr_xfer_read_txs /\ spi.state = xfer_channel_enabled) \/
 (dr.state = dr_xfer_check_txs /\ spi.state = xfer_channel_enabled))) /\
@@ -109,6 +114,7 @@ IS_STATE_REL (ds_abs1:ds_abs1_state) (dr:driver_state) (spi:spi_state) =
 (dr.state = dr_xfer_fetch_dataI /\ spi.state = xfer_ready_for_trans)) /\
 ((ds_abs1.state = abs1_xfer_reset) =
 ((dr.state = dr_xfer_issue_disable /\ spi.state = xfer_ready_for_trans) \/
+(dr.state = dr_xfer_read_conf /\ spi.state = xfer_channel_disabled) \/
 (dr.state = dr_xfer_reset_conf /\ spi.state = xfer_channel_disabled))))`
 
 (* ref_rel: refinement relation for the ds_abs1 and (dr,spi). *)
@@ -160,24 +166,39 @@ ref_rel (ds_abs1:ds_abs1_state) (dr:driver_state, spi:spi_state) =
 (0 >< 0) (THE dr.dr_last_read_v) = 0w:word1) /\
 (spi.state = init_reset ==> spi.regs.SYSSTATUS = 0w) /\
 (spi.state = init_setregs ==> spi.regs.SYSSTATUS = 1w) /\
+(spi.state = init_setregs ==> spi.regs.CH0CONF.FORCE = 0w /\
+spi.regs.CH0CONF.IS = 1w /\ spi.regs.CH0CONF.DPE1 = 1w /\
+spi.regs.CH0CONF.DPE0 = 0w /\ spi.regs.CH0CONF.TRM = 0w /\
+spi.regs.CH0CONF.WL = 0w /\ spi.regs.CH0CONF.EPOL = 0w /\
+spi.regs.CH0CONF.CLKD = 0w /\ spi.regs.CH0CONF.POL = 0w /\
+spi.regs.CH0CONF.PHA = 0w) /\
+(spi.state = spi_ready ==> spi.regs.CH0CONF.FORCE = 0w) /\
+(spi.state = tx_conf_ready \/ spi.state = tx_channel_enabled \/
+spi.state = tx_ready_for_trans \/ spi.state = tx_trans_data \/
+spi.state = tx_trans_done \/ spi.state = tx_trans_next \/
+spi.state = tx_trans_update \/ spi.state = tx_channel_disabled \/
+spi.state = rx_conf_ready \/ spi.state = rx_channel_enabled \/ 
+spi.state = rx_receive_data \/ spi.state = rx_update_RX0 \/
+spi.state = rx_data_ready \/ spi.state = rx_channel_disabled \/
+spi.state = xfer_conf_ready \/ spi.state = xfer_channel_enabled \/ 
+spi.state = xfer_ready_for_trans \/ spi.state = xfer_trans_data \/
+spi.state = xfer_exchange_data \/ spi.state = xfer_update_RX0 \/
+spi.state = xfer_data_ready \/ spi.state = xfer_channel_disabled ==>
+spi.regs.CH0CONF.FORCE = 1w) /\
 ((dr.state = dr_init_read_req /\ spi.state = init_reset) \/
 (dr.state = dr_init_check_rep /\ spi.state = init_reset) \/
 (dr.state = dr_init_read_req /\ spi.state = init_setregs) \/
 (dr.state = dr_init_check_rep /\ spi.state = init_setregs) ==>
-~ dr.dr_init.issue_wr_sysconfig /\ ~ dr.dr_init.issue_wr_modulctrl /\
-~ dr.dr_init.issue_wr_ch0conf_wl /\ ~ dr.dr_init.issue_wr_ch0conf_mode /\
-~ dr.dr_init.issue_wr_ch0conf_speed /\ ~ spi.init.sysconfig_mode_done /\ 
-~ spi.init.modulctrl_bus_done /\ ~ spi.init.ch0conf_wordlen_done /\ 
-~ spi.init.ch0conf_mode_done /\ ~ spi.init.ch0conf_speed_done) /\
+~ dr.dr_init.issue_wr_sysconfig /\ ~ dr.dr_init.issue_wr_modulctrl /\ 
+~ spi.init.sysconfig_mode_done /\ ~ spi.init.modulctrl_bus_done) /\
 (dr.dr_init.issue_wr_sysconfig = spi.init.sysconfig_mode_done) /\
 (dr.dr_init.issue_wr_modulctrl = spi.init.modulctrl_bus_done) /\
-(dr.dr_init.issue_wr_ch0conf_wl = spi.init.ch0conf_wordlen_done) /\
-(dr.dr_init.issue_wr_ch0conf_mode = spi.init.ch0conf_mode_done) /\
-(dr.dr_init.issue_wr_ch0conf_speed = spi.init.ch0conf_speed_done) /\
 (~ dr.dr_init.issue_wr_sysconfig ==> ~ dr.dr_init.issue_wr_modulctrl) /\
-(~ dr.dr_init.issue_wr_modulctrl ==> ~ dr.dr_init.issue_wr_ch0conf_wl) /\
-(~ dr.dr_init.issue_wr_ch0conf_wl ==> ~ dr.dr_init.issue_wr_ch0conf_mode) /\
-(~ dr.dr_init.issue_wr_ch0conf_mode ==> ~ dr.dr_init.issue_wr_ch0conf_speed) /\
+(* for CH0CONF *)
+(dr.state = dr_tx_fetch_conf \/ dr.state = dr_tx_reset_conf \/ 
+dr.state = dr_rx_fetch_conf \/ dr.state = dr_rx_reset_conf \/ 
+dr.state = dr_xfer_fetch_conf \/ dr.state = dr_xfer_reset_conf ==> 
+dr.dr_last_read_v = SOME (build_CH0CONF spi.regs.CH0CONF)) /\
 (* for tx automaton *)
 (spi.state = tx_channel_enabled /\ dr.state = dr_tx_check_txs ==>
 (1 >< 1) (THE dr.dr_last_read_v) = 0w:word1) /\
