spi_model/SPI_update_regsScript.sml
@@ -13,18 +13,12 @@ spi with <| regs := spi.regs with
 <| SYSCONFIG := spi.regs.SYSCONFIG with SOFTRESET := 0w; (* automatically reset by hardware *)
 SYSSTATUS := 0w |>;
 state := init_reset;
-init := spi.init with 
-<| sysconfig_mode_done := F; modulctrl_bus_done := F; 
-ch0conf_wordlen_done := F; ch0conf_mode_done := F;
-ch0conf_speed_done := F |> |>
+init := <| sysconfig_mode_done := F; modulctrl_bus_done := F |> |>
 else if (spi.state = spi_ready) /\ (v = 1w) then
 spi with <| regs := spi.regs with 
 <|SYSCONFIG := spi.regs.SYSCONFIG with SOFTRESET := 0w; SYSSTATUS := 0w |>;
 state := init_reset;
-init := spi.init with 
-<| sysconfig_mode_done := F; modulctrl_bus_done:= F; 
-   ch0conf_wordlen_done := F; ch0conf_mode_done := F;
-   ch0conf_speed_done := F |> |>
+init := <| sysconfig_mode_done := F; modulctrl_bus_done := F |> |>
 else spi with err := T (* SPI is not ready to reset *)`
 
 (* write_SYSCONFIG: write a value to spi.regs.SYSCONFIG, set some bits of SYSCONFIG. *)
@@ -37,8 +31,7 @@ spi with <| regs := spi.regs with
 SYSCONFIG := spi.regs.SYSCONFIG with <|SIDLEMODE := 2w; AUTOIDLE := 1w |>;
 init := spi.init with sysconfig_mode_done := T;
 state := 
-if (spi.init.modulctrl_bus_done /\ spi.init.ch0conf_wordlen_done 
-/\ spi.init.ch0conf_mode_done /\ spi.init.ch0conf_speed_done) 
+if spi.init.modulctrl_bus_done /\ spi.regs.CH0CONF.WL >+ 2w 
 then spi_ready else init_setregs |> 
 else spi with err := T`
 
@@ -62,58 +55,106 @@ spi with <| regs := spi.regs with MODULCTRL := spi.regs.MODULCTRL with
 <| SYSTEM_TEST := v3; MS := v2; SINGLE := v1 |>;
 init := spi.init with modulctrl_bus_done := T;
 state := 
-if (spi.init.sysconfig_mode_done /\ spi.init.ch0conf_wordlen_done 
-/\ spi.init.ch0conf_mode_done /\ spi.init.ch0conf_speed_done) 
+if spi.init.sysconfig_mode_done /\ spi.regs.CH0CONF.WL >+ 2w
 then spi_ready else init_setregs |> 
 else spi with err := T`
 
-(* write_CH0CONF_WL: set a value to spi.regs.CH0CONF with WL(word length) bit. *)
-val write_CH0CONF_WL_def = Define `
-write_CH0CONF_WL (value:word32) (spi:spi_state) =
-let v = (11 >< 7) value:word5 in
-if (spi.state = init_setregs) /\ (v >+ 2w) (* Bit WL should be bigger than 2w *) then 
-spi with <| regs := spi.regs with 
-CH0CONF := spi.regs.CH0CONF with WL := v;
-init := spi.init with ch0conf_wordlen_done := T;
-state := 
-if (spi.init.sysconfig_mode_done /\ spi.init.modulctrl_bus_done 
-/\ spi.init.ch0conf_mode_done /\ spi.init.ch0conf_speed_done) 
-then spi_ready else init_setregs |> 
+
+(* write_CH0CONF_tx: write a value to spi.regs.CH0CONF to start and finish the tx mode, vaild when TRM = 2. *)
+val write_CH0CONF_tx_def = Define `
+write_CH0CONF_tx (value:word32) (spi:spi_state) =
+let v0 = (20 >< 20) value:word1 and
+    v4 = (13 >< 12) value:word2 in
+if (spi.state = spi_ready) /\ (v0 = 1w) then 
+spi with <| regs := spi.regs with CH0CONF := spi.regs.CH0CONF
+with <|TRM := 2w; FORCE := 1w |>;
+state := tx_conf_ready |> 
+else if (spi.state = tx_channel_disabled) /\ (v0 = 0w) /\ (v4 = spi.regs.CH0CONF.TRM) then
+spi with <| regs := spi.regs with CH0CONF := spi.regs.CH0CONF with FORCE := 0w;
+state := spi_ready |> 
 else spi with err := T`
 
-(* write_CH0CONF: set a value to spi.regs.CH0CONF for some bits, including IS, DPE1, DPE0, TRM, EPOL, POL, PHA. *)
-val write_CH0CONF_def = Define `
-write_CH0CONF (value:word32) (spi:spi_state) =
+(* write_CH0CONF_rx: write the spi.regs.CH0CONF to start and finish the rx mode, vaild when TRM = 1. *)
+val write_CH0CONF_rx_def = Define `
+write_CH0CONF_rx (value:word32) (spi:spi_state) =
+let v0 = (20 >< 20) value:word1 and
+    v4 = (13 >< 12) value:word2 in
+if (spi.state = spi_ready) /\ (v0 = 1w) then
+spi with <| regs := spi.regs with CH0CONF := spi.regs.CH0CONF
+with <|TRM := 1w; FORCE := 1w|>;
+state := rx_conf_ready |>
+else if (spi.state = rx_channel_disabled) /\ (v0 = 0w) /\ (v4 = spi.regs.CH0CONF.TRM) then 
+spi with <| regs := spi.regs with CH0CONF := spi.regs.CH0CONF with FORCE := 0w;
+state := spi_ready |> 
+else spi with err := T`
+
+(* write_CH0CONF_xfer: write the spi.regs.CH0CONF to start and finish the xfer mode, vaild when TRM = 0. *)
+val write_CH0CONF_xfer_def = Define `
+write_CH0CONF_xfer (value:word32) (spi:spi_state) =
+let v0 = (20 >< 20) value:word1 and
+    v4 = (13 >< 12) value:word2 in
+if (spi.state = spi_ready) /\ (v0 = 1w) then
+spi with <| regs := spi.regs with CH0CONF := spi.regs.CH0CONF
+with  <| TRM := 0w; FORCE := 1w |>;
+state := xfer_conf_ready |> 
+else if (spi.state = xfer_channel_disabled) /\ (v0 = 0w) /\ (v4 = spi.regs.CH0CONF.TRM) then
+spi with <| regs := spi.regs with CH0CONF := spi.regs.CH0CONF  with FORCE := 0w;
+state := spi_ready |> 
+else spi with err := T`
+
+(* ch0conf_changed: check if the value wants to change the configuration or not *)
+val ch0conf_changed_def = Define `
+ch0conf_changed (value:word32) (spi:spi_state) =
 let v1 = (18 >< 18) value:word1 and
     v2 = (17 >< 17) value:word1 and
     v3 = (16 >< 16) value:word1 and
+    v5 = (11 >< 7) value:word5 and
+    v6 = (6 >< 6) value:word1 and
+    v7 = (5 >< 2) value:word4 and
+    v8 = (1 >< 1) value:word1 and
+    v9 = (0 >< 0) value:word1 in
+~ ((v1 = spi.regs.CH0CONF.IS) /\ (v2 = spi.regs.CH0CONF.DPE1) /\
+   (v3 = spi.regs.CH0CONF.DPE0) /\ (v5 = spi.regs.CH0CONF.WL) /\
+   (v6 = spi.regs.CH0CONF.EPOL) /\ (v7 = spi.regs.CH0CONF.CLKD) /\
+   (v8 = spi.regs.CH0CONF.POL) /\ (v9 = spi.regs.CH0CONF.PHA))`
+
+(* write_CH0CONF_init: set baisc values *)
+val write_CH0CONF_init_def = Define `
+write_CH0CONF_init (value:word32) (spi:spi_state) =
+let v0 = (20 >< 20) value:word1 and
+    v1 = (18 >< 18) value:word1 and
+    v2 = (17 >< 17) value:word1 and
+    v3 = (16 >< 16) value:word1 and
     v4 = (13 >< 12) value:word2 and
-    v5 = (6 >< 6) value:word1 and
-    v6 = (1 >< 1) value:word1 and
-    v7 = (0 >< 0) value:word1 in
-if (spi.state = init_setregs) /\ (v4 <> 3w) then 
-spi with <|regs := spi.regs with CH0CONF := spi.regs.CH0CONF with 
-<| IS := v1; DPE1 := v2; DPE0 := v3;
-TRM := v4; EPOL := v5; POL := v6; PHA := v7 |>;
-init := spi.init with ch0conf_mode_done := T;
-state := 
-if (spi.init.sysconfig_mode_done /\ spi.init.modulctrl_bus_done 
-/\ spi.init.ch0conf_wordlen_done /\ spi.init.ch0conf_speed_done) 
+    v5 = (11 >< 7) value:word5 and
+    v6 = (6 >< 6) value:word1 and
+    v7 = (5 >< 2) value:word4 and
+    v8 = (1 >< 1) value:word1 and
+    v9 = (0 >< 0) value:word1 in
+if (spi.state = init_setregs \/ spi.state = spi_ready) /\ (v4 <> 3w) /\ (v0 = spi.regs.CH0CONF.FORCE) then 
+spi with <|regs := spi.regs with 
+CH0CONF := spi.regs.CH0CONF with <| IS := v1; DPE1 := v2; DPE0 := v3; TRM := v4; WL:= v5; 
+EPOL := v6; CLKD := v7; POL := v8; PHA := v9 |>;
+state := if v5 >+ 2w /\ spi.init.sysconfig_mode_done /\ spi.init.modulctrl_bus_done
 then spi_ready else init_setregs |>
 else spi with err := T`
 
-(* write_CH0CONF_speed: write a value to spi.regs.CH0CONF to set speed. *)
-val write_CH0CONF_speed_def = Define `
-write_CH0CONF_speed (value:word32) (spi:spi_state) =
-let v = (5 >< 2) value:word4 in
-if spi.state = init_setregs then
-spi with <|regs := spi.regs with
-CH0CONF := spi.regs.CH0CONF with CLKD := v;
-init := spi.init with ch0conf_speed_done := T;
-state := 
-if (spi.init.sysconfig_mode_done /\ spi.init.modulctrl_bus_done 
-/\ spi.init.ch0conf_wordlen_done /\ spi.init.ch0conf_mode_done)
-then spi_ready else init_setregs |>
+(* write_CH0CONF_comb: a general function for update the CH0CONF register *)
+val write_CH0CONF_comb_def = Define `
+write_CH0CONF_comb (value:word32) (spi:spi_state) =
+if ch0conf_changed value spi then write_CH0CONF_init value spi
+else if ((20 >< 20) value:word1 <> spi.regs.CH0CONF.FORCE) /\
+(((13 >< 12) value:word2 = 2w /\ spi.state = spi_ready) \/
+(spi.state = tx_channel_disabled))
+then write_CH0CONF_tx value spi
+else if ((20 >< 20) value:word1 <> spi.regs.CH0CONF.FORCE) /\
+(((13 >< 12) value:word2 = 1w /\ spi.state = spi_ready) \/
+(spi.state = rx_channel_disabled))
+then write_CH0CONF_rx value spi
+else if ((20 >< 20) value:word1 <> spi.regs.CH0CONF.FORCE) /\
+(((13 >< 12) value:word2 = 0w /\ spi.state = spi_ready) \/
+(spi.state = xfer_channel_disabled))
+then write_CH0CONF_xfer value spi
 else spi with err := T`
 
 (* write_CH0CTRL: enable or disable the SPI channel. *)
@@ -141,70 +182,6 @@ then spi with <|regs := spi.regs with
 else if (spi.state = xfer_ready_for_trans) /\ (v = 0w)
 then spi with <|regs := spi.regs with CH0CTRL := 0w;
      state := xfer_channel_disabled |>
-else spi with err := T`
-
-
-(* write_CH0CONF_tx: write a value to spi.regs.CH0CONF to start and finish the tx mode, vaild when TRM = 2. *)
-val write_CH0CONF_tx_def = Define `
-write_CH0CONF_tx (value:word32) (spi:spi_state) =
-let v1 = (13 >< 12) value:word2 and
-    v2 = (20 >< 20) value:word1 in
-if (spi.state = spi_ready) /\ (v1 = 2w) /\ (v2 = 1w) then 
-spi with <| regs := spi.regs with CH0CONF := spi.regs.CH0CONF
-with <|TRM := 2w; FORCE := 1w |>;
-state := tx_conf_ready |> 
-else if (spi.state = tx_channel_disabled) /\ (v2 = 0w) then
-spi with <| regs := spi.regs with CH0CONF := spi.regs.CH0CONF with FORCE := 0w;
-state := spi_ready |> 
-else spi with err := T`
-
-(* write_CH0CONF_rx: write the spi.regs.CH0CONF to start and finish the rx mode, vaild when TRM = 1. *)
-val write_CH0CONF_rx_def = Define `
-write_CH0CONF_rx (value:word32) (spi:spi_state) =
-let v1 = (13 >< 12) value:word2 and
-    v2 = (20 >< 20) value:word1 in
-if (spi.state = spi_ready) /\ (v1 = 1w) /\ (v2 = 1w) then
-spi with <| regs := spi.regs with CH0CONF := spi.regs.CH0CONF
-with <|TRM := 1w; FORCE := 1w|>;
-state := rx_conf_ready |>
-else if (spi.state = rx_channel_disabled) /\ (v2 = 0w) then
-spi with <| regs := spi.regs with CH0CONF := spi.regs.CH0CONF with FORCE := 0w;
-state := spi_ready |> 
-else spi with err := T`
-
-(* write_CH0CONF_xfer: write the spi.regs.CH0CONF to start and finish the xfer mode, vaild when TRM = 0. *)
-val write_CH0CONF_xfer_def = Define `
-write_CH0CONF_xfer (value:word32) (spi:spi_state) =
-let v1 = (13 >< 12) value:word2 and
-    v2 = (20 >< 20) value:word1 in
-if (spi.state = spi_ready) /\ (v1 = 0w) /\ (v2 = 1w) then
-spi with <| regs := spi.regs with CH0CONF := spi.regs.CH0CONF
-with  <| TRM := 0w; FORCE := 1w |>;
-state := xfer_conf_ready |> 
-else if (spi.state = xfer_channel_disabled) /\ (v2 = 0w) then
-spi with <| regs := spi.regs with CH0CONF := spi.regs.CH0CONF  with FORCE := 0w;
-state := spi_ready |> 
-else spi with err := T`
-
-(* write_CH0CONF_comb: combine the functions updateing the CH0CONF register *)
-val write_CH0CONF_comb_def = Define `
-write_CH0CONF_comb (value:word32) (spi:spi_state) =
-if ((11 >< 7) value:word5 <> spi.regs.CH0CONF.WL) 
-then (write_CH0CONF_WL value spi) 
-else if ((17 >< 17) value:word1 <> spi.regs.CH0CONF.DPE1 /\ 
-(16 >< 16) value: word1 <> spi.regs.CH0CONF.DPE0) 
-then (write_CH0CONF value spi) 
-else if ((5 >< 2) value:word4 <> spi.regs.CH0CONF.CLKD) 
-then (write_CH0CONF_speed value spi) 
-else if ((13 >< 12) value:word2 = 2w) \/ 
-((20 >< 20) value:word1 <> spi.regs.CH0CONF.FORCE /\ spi.state = tx_channel_disabled)
-then (write_CH0CONF_tx value spi)
-else if ((13 >< 12) value:word2 = 1w) \/ 
-((20 >< 20) value:word1 <> spi.regs.CH0CONF.FORCE /\ spi.state = rx_channel_disabled)
-then (write_CH0CONF_rx value spi) 
-else if ((13 >< 12) value:word2 = 0w) \/ 
-((20 >< 20) value:word1 <> spi.regs.CH0CONF.FORCE /\ spi.state = xfer_channel_disabled) 
-then (write_CH0CONF_xfer value spi)
 else spi with err := T`
 
 (* write_TX0: write a byte (data) to TX0 register, and clear the TXS Bit. *)
